\chapter{Derivation of the algorithm for updating the inverse Slater matrix}\label{updatingAlgorithmDer}  % use *-form to suppress numbering

\renewcommand{\theequation}{A-\arabic{equation}}
  
 \setcounter{equation}{0}  % reset counter 

The following derivation follows the ideas given in Ref.\cite{Williansom}. As starting point we may consider that each time a new position is suggested in the Metropolis algorithm, a row of the current Slater matrix experiences some kind of perturbation. Hence, the Slater matrix with its orbitals evaluated at the new position equals the old Slater matrix plus a perturbation matrix,

\begin{equation}\label{oldSM}
D_{jk}(\bfv{x^{new}}) = D_{jk}(\bfv{x^{cur}}) + \Delta_{jk}.
\end{equation}

where

\begin{equation}\label{pertMatrix}
\Delta_{jk} = \delta_{ik}[\phi_j(\bfv{x_{i}^{new}}) - \phi_j(\bfv{x_{i}^{old}})] = \delta_{ik}(\Delta\phi)_j 
\end{equation}

Computing $(B^T)^{-1}$ we arrive to

\begin{equation}\label{invDkj}
 D_{kj}(\bfv{x^{new}})^{-1} = [D_{kj}(\bfv{x^{cur}}) + \Delta_{kj}]^{-1}.
\end{equation}

The evaluation of the right hand side (rhs) term above is carried out by applying the identity $(A +  B)^{-1} = A^{-1} - (A + B)^{-1} B A^{-1}$. In compact notation it yields

\begin{eqnarray*}
 [\bfv{D}^{T}(\bfv{x^{new}})]^{-1} & = & [\bfv{D}^{T}(\bfv{x^{cur}}) + \Delta^T]^{-1}\\
& = & [\bfv{D}^{T}(\bfv{x^{cur}})]^{-1} - [\bfv{D}^{T}(\bfv{x^{cur}}) + \Delta^T]^{-1} \Delta^T [\bfv{D}^{T}(\bfv{x^{cur}})]^{-1}\\
& = & [\bfv{D}^{T}(\bfv{x^{cur}})]^{-1} - \underbrace{{[\bfv{D}^{T}(\bfv{x^{new}})]^{-1}}}_{\text{By Eq.}{\ref{invDkj}}}  \Delta^T [\bfv{D}^{T}(\bfv{x^{cur}})]^{-1}.
\end{eqnarray*}

Using index notation, the last result may be expanded by
% % % % % % % [D^{T}_{jk}(\bfv{x^{new}})]^{-1} & = & [D^{T}_{jk}(\bfv{x^{cur}})]^{-1} +  \sum_{l} \sum_{m} [D^{T}_{mk}(\bfv{x^{new}})]^{-1} \Delta^{T}_{ml}  [D^{T}_{jl}(\bfv{x^{cur}})]^{T}\\


\begin{eqnarray*}
D^{-1}_{kj}(\bfv{x^{new}}) & = & D^{-1}_{kj}(\bfv{x^{cur}}) -  \sum_{l} \sum_{m} D^{-1}_{km}(\bfv{x^{new}}) \Delta^{T}_{ml}  D^{-1}_{lj}(\bfv{x^{cur}})\\
& = & D^{-1}_{kj}(\bfv{x^{cur}}) -  \sum_{l} \sum_{m} D^{-1}_{km}(\bfv{x^{new}}) \Delta_{lm}  D^{-1}_{lj}(\bfv{x^{cur}})\\
& = & D^{-1}_{kj}(\bfv{x^{cur}}) -  \sum_{l} \sum_{m} D^{-1}_{km}(\bfv{x^{new}}) \underbrace{\delta_{im} (\Delta \phi)_{l}}_{\text{By Eq. }\ref{pertMatrix}}  D^{-1}_{lj}(\bfv{x^{cur}})\\
& = & D^{-1}_{kj}(\bfv{x^{cur}}) - D^{-1}_{ki}(\bfv{x^{new}}) \sum_{l=1}^{N}(\Delta \phi)_{l}  D^{-1}_{lj}(\bfv{x^{cur}})\\
& = & D^{-1}_{kj}(\bfv{x^{cur}}) - D^{-1}_{ki}(\bfv{x^{new}}) \sum_{l=1}^{N}\underbrace{[\phi_{l}(\bfv{r_{i}^{new}}) - \phi_{l}(\bfv{r_{i}^{old}})]}_{\text{By Eq.}\ref{pertMatrix}}  D^{-1}_{lj}(\bfv{x^{cur}}).
\end{eqnarray*}

From (\ref{inverseDef}), 

$$\bfv{D}^{-1}(\bfv{x^{cur}}) = \frac{adj \bfv{D}}{|\bfv{D}(\bfv{x^{cur}})|} \, \quad \text{and} \, \quad \bfv{D}^{-1}(\bfv{x^{new}}) = \frac{adj \bfv{D}}{|\bfv{D}(\bfv{x^{new}})|}.$$

Dividing these two equations we get

$$\frac{\bfv{D}^{-1}(\bfv{x^{cur}})}{\bfv{D}^{-1}(\bfv{x^{new}})} = \frac{|\bfv{D}(\bfv{x^{new}})|}{|\bfv{D}(\bfv{x^{cur}})|} = R \Rightarrow D^{-1}_{ki}(\bfv{x^{new}}) = \frac{D^{-1}_{ki}(\bfv{x^{cur}})}{R}.$$

Therefore,

$$D^{-1}_{kj}(\bfv{x^{new}})  =  D^{-1}_{kj}(\bfv{x^{cur}}) - \frac{D^{-1}_{ki}(\bfv{x^{cur}})}{R} \sum_{l=1}^{N}[\phi_{l}(\bfv{r_{i}^{new}}) - \phi_{l}(\bfv{r_{i}^{old}})]  D^{-1}_{lj}(\bfv{x^{cur}}),$$

or

\begin{align}
 D^{-1}_{kj}(\bfv{x^{new}})  =  D^{-1}_{kj}(\bfv{x^{cur}}) \qquad & - & \frac{D^{-1}_{ki}(\bfv{x^{cur}})}{R} \sum_{l=1}^{N}\phi_{l}(\bfv{r_{i}^{new}})  D^{-1}_{lj}(\bfv{x^{cur}}) \nonumber\\
  & + &  \frac{D^{-1}_{ki}(\bfv{x^{cur}})}{R} \sum_{l=1}^{N}\phi_{l}(\bfv{r_{i}^{old}})  D^{-1}_{lj}(\bfv{x^{cur}})\nonumber\\
                             =  D^{-1}_{kj}(\bfv{x^{cur}}) \qquad & - & \frac{D^{-1}_{ki}(\bfv{x^{cur}})}{R} \sum_{l=1}^{N} D_{il}(\bfv{x^{new}})  D^{-1}_{lj}(\bfv{x^{cur}}) \nonumber\\
& + &  \frac{D^{-1}_{ki}(\bfv{x^{cur}})}{R} \sum_{l=1}^{N} D_{il}(\bfv{x^{cur}}) D^{-1}_{lj}(\bfv{x^{cur}}).\nonumber
\end{align}

% % % % & = & D^{-1}_{kj}(\bfv{x^{cur}}) - \frac{S_j}{R} D^{-1}_{ki}(\bfv{x^{cur}})
In this equation, the first line becomes zero for $j=i$ and the second for $j \neq i$. Therefore, the update of the inverse for the new Slater matrix is given by

\begin{eqnarray}
\boxed{D^{-1}_{kj}(\bfv{x^{new}})  = \left\{ 
\begin{array}{l l}
  D^{-1}_{kj}(\bfv{x^{cur}}) - \frac{D^{-1}_{ki}(\bfv{x^{cur}})}{R} \sum_{l=1}^{N} D_{il}(\bfv{x^{new}})  D^{-1}_{lj}(\bfv{x^{cur}}) & \mbox{if $j \neq i$}\nonumber \\ \\
 \frac{D^{-1}_{ki}(\bfv{x^{cur}})}{R} \sum_{l=1}^{N} D_{il}(\bfv{x^{cur}}) D^{-1}_{lj}(\bfv{x^{cur}}) & \mbox{if $j=i$}
\end{array} \right.}
\end{eqnarray}

\clearemptydoublepage
