\documentclass{article}
\usepackage[svgnames]{xcolor}
\usepackage{amsmath}
\usepackage[most]{tcolorbox}
\usepackage[margin=1in]{geometry} 

\begin{document}
We have 

\begin{equation}
\label{eq:dvdt}
    \frac{\partial V}{\partial t}=\nabla \cdot (\mathbf{\sigma}_m \nabla V) - kV(V-a)(V-1)-VW,
\end{equation}
and
\begin{equation}
\label{dwdt}
    \frac{\partial W}{\partial t}= (\epsilon + \frac{\mu_1W}{V+\mu_2})(-W-kV(V-b-1)).
\end{equation}
\\

Rescaling $x$,$y$ and $t$ such that

\begin{equation}
    \Tilde{x}=\alpha x,\: \Tilde{y}=\alpha y,\: \text{and}\: \Tilde{t}=\beta t,
\end{equation}



where $\alpha$ and $\beta$ are constant scaling factors, we get



\begin{equation}
    \frac{\partial x}{\partial \Tilde{x}} = \frac{1}{\alpha},\: \frac{\partial y}{\partial \Tilde{y}} = \frac{1}{\alpha}\: \text{and}\: \frac{\partial t}{\partial \Tilde{t}} = \frac{1}{\beta}.
\end{equation}

Using the chain rule, we get

\begin{equation}
    \frac{\partial V}{\partial \Tilde{x}}=\frac{\partial x}{\partial \Tilde{x}}\frac{\partial V}{\partial x} \rightarrow \frac{\partial V}{\partial x}=\alpha \frac{\partial V}{\partial \Tilde{x}},
\end{equation}

\begin{equation}
    \frac{\partial V}{\partial \Tilde{y}}=\frac{\partial y}{\partial \Tilde{y}}\frac{\partial V}{\partial y} \rightarrow \frac{\partial V}{\partial y}= \alpha \frac{\partial V}{\partial \Tilde{y}},
\end{equation}
and 
\begin{equation}
    \frac{\partial V}{\partial \Tilde{t}}=\frac{\partial t}{\partial \Tilde{t}}\frac{\partial V}{\partial t} \rightarrow \frac{\partial V}{\partial t} = \beta \frac{\partial V}{\partial \Tilde{t}}.
\end{equation}
\\

Similarly, we get $\frac{\partial \sigma(x,y)}{\partial x} = \alpha \frac{\partial \sigma(x,y)}{\partial \Tilde{x}}$ and $\frac{\partial \sigma(x,y)}{\partial y} = \alpha \frac{\partial \sigma(x,y)}{\partial \Tilde{y}}$.\\

Thus, we can write \eqref{eq:dvdt} and \eqref{dwdt} as
\begin{equation}
\label{eq:dvdt}
    \beta \frac{\partial V}{\partial \Tilde{t}}=\alpha^2\Tilde{\nabla} \cdot (\mathbf{\sigma}_m \Tilde{\nabla} V) - kV(V-a)(V-1)-VW,
\end{equation}
and
\begin{equation}
\label{dwdt}
    \beta \frac{dW}{d \Tilde{t}}= (\epsilon + \frac{\mu_1W}{V+\mu_2})(-W-kV(V-b-1)).
\end{equation}


\end{document}